\documentclass[12pt]{article}
\usepackage{amsmath}
\usepackage{graphicx}
\usepackage{hyperref}
\usepackage[latin1]{inputenc}

\begin{document}

$y_{nk}=\frac{e^{{w_k^{(2)}}^T}\cdot z_n}{\sum_{j}^{K}e^{{w_j^{(2)}}^T}\cdot z_n}$
$a_{nk}= {w_k^{(2)}}^T \cdot z_n $

$E(x)= \sum_{n=1}^{Nb}\sum_{k=1}^{K}t_{nk}\cdot \log(y_{nk}) - \frac{\lambda}{2} \cdot \Vert w_k^{(2)}\Vert^2 \\
=\sum_{n=1}^{Nb}\sum_{k=1}^{K}t_{nk}\cdot \log\bigg(\frac{e^{{w_k^{(2)}}^T\cdot z_n}}{\sum_{j}^{K}e^{{w_j^{(2)}}^T}\cdot z_n}\bigg) - \frac{\lambda}{2} \cdot \Vert w_k^{(2)}\Vert^2 \\
=\sum_{n=1}^{Nb}\sum_{k=1}^{K} t_{nk} \cdot \big[{w_k^{(2)}}^T \cdot z_n - \log\big(\sum_{j}^{K}e^{{w_j^{(2)}}^T\cdot z_n} \big)\big] - \frac{\lambda}{2} \cdot \Vert w_k^{(2)}\Vert^2 \\
=\sum_{n=1}^{Nb}\sum_{k=1}^{K} \big[ t_{nk} \cdot a_{nk} - t_{nk} \cdot \log\big( \sum_{j}^{K}e^{a_{nj}} \big) \big] - \frac{\lambda}{2} \cdot \Vert w_k^{(2)}\Vert^2 \\
$

$
E_n=\sum_{k=1}^{K}t_{nk} \cdot a_{nk} -\sum_{k=1}^{K} t_nk \cdot \log \big(\sum_{j}^{K}e^{a_{nj}}\big) \\
=\sum_{k!=p}^K t_{nk} \cdot a_{nk} + t_{np} \cdot a_{np} - \sum_{k!=p}^K t_{nk} \cdot \log \big( \sum_j^K e^{a_{nj}}\big) - t_{np} \cdot \log \big( \sum_j^K e^{a_{nj}} \big)\\
$

$
\frac{\delta E_n}{\delta a_{np}}=\frac{\delta\big[ \sum_{k!=p}^K t_{nk} \cdot a_{nk}  \big]}{\delta a_{np}} + \frac{\delta \big[t_{np} \cdot a_{np}\big]}{\delta a_{np}} - \frac{\delta \big [ \sum_{k!=p}^K t_{nk} \cdot \log (\sum_j^Ke^{a_{nj}}) \big]}{\delta a_{np}} - \frac{\delta \big [ t_{np} \cdot \log (\sum_j^Ke^{a_{nj}}) \big]}{\delta a_{np}} \\
= t_{np} - \Big(\frac{e^{a_{np}}}{\sum_{j}^{K}e^{a_{nj}}}\Big) \cdot \sum_{k!=p}^K t_{nk} - t_{np} \cdot \Big( \frac{e^{a_{np}}}{\sum_j^Ke^{a_{nj}}} \Big) \\
= t_{np} - y_{nk} \cdot \sum_{k=1}^K t_{nk} = t_{np} - y_{np} \\
$

$
\frac{\delta a_{np}}{\delta z_{nq}} = \frac{\delta[{w_{p}^{(2)}}^T \cdot z_{n}]}{\delta z_{nq}} = \frac {\delta [\sum_j^{M+1}w_{pj}^{(2)} \cdot z_{nj}]}{\delta z_{nq}} = w_{pq}^{(2)}
$

$
\frac{\delta E_n}{\delta z_{nq}} = \frac{\delta E_n}{\delta a_{np}} \cdot \frac{\delta a_{np}}{\delta z_{nq}} = \big( t_{np} - y_{np} \big) \cdot w_{pq}^{(2)}
$

$
o_{nj} = {w_j^{(1)}}^T \cdot x_n 
$

$
h3 \\
z_{nj} = \cos(o_{nj})
$

$
\frac{\delta z_{nq}}{\delta o_{nq}} = \frac{\delta [\cos(o_{nq})]}{\delta o_{nq}} = -\sin{(o_{nq})}
$

$
\frac{\delta o_{nq}}{\delta w_{qm}^{(1)}} = \frac{\delta [{w_q^{(1)}}^T \cdot x_n]}{\delta w_{qm}^{(1)}} = x_{nm}
$

$
\frac{\delta E_n}{\delta w_{qm}^{(1)}} = \frac{\delta E_n}{\delta z_{nq}} \cdot \frac{\delta z_{nq}}{\delta o_{nq}} \cdot \frac{\delta o_{nq}}{\delta w_{qm}^{(1)}} \\
= \big( t_{np} - y_{np} \big) \cdot w_{pq}^{(2)} \cdot \big(-\sin{(o_{nq})}\big) \cdot x_{nm} \\
= \big( t_{np} - y_{np} \big) \cdot w_{pq}^{(2)} \cdot \big(-\sin{({w_q^{(1)}}^T \cdot x_n)}\big) \cdot x_{nm} \\
... \\
= {((T - Y) \cdot W^{(2)})}^T \cdot (-\sin (K)) \cdot X
$





\end{document}